

# Solution manual - Scattering theory - Taylor

zlatomir.zhelev04

August 2025

# Contents

## Chapter 2

## Chapter 3

## Chapter 4

### Problem 4.1

We can write:

$$d\Omega = 2\pi d(\cos \theta)$$

From this we have to calculate:

$$\frac{d\Omega_{cm}}{d\Omega_{lab}} = \frac{d(\cos \theta_{cm})}{d(\cos \theta_{lab})} = \frac{1}{\frac{d(\cos \theta_{lab})}{d(\cos \theta_{cm})}}$$

Thus we have to find  $\cos \theta_{lab}$  as a function of  $\cos \theta_{cm}$ . We can do this by using a formula such as one that can be seen in Landau & Lifschitz, Vol 1. Mechanics, which gives us:

$$\tan \theta_{lab} = \frac{\sin \theta_{cm}}{\lambda + \cos \theta_{cm}}$$

Here  $\lambda = \frac{m_1}{m_2}$  as in Taylor's text. We square the equation and obtain:

$$\begin{aligned} \tan^2 \theta_{lab} &= \frac{1}{\cos^2 \theta_{lab}} - 1 = \frac{1 - \cos^2 \theta_{cm}}{(\lambda + \cos \theta_{cm})^2} \\ \Rightarrow \frac{1}{\cos^2 \theta_{lab}} &= \frac{1 - \cos^2 \theta_{cm} + \cos^2 \theta_{cm} + 2\lambda \cos \theta_{cm} + \lambda^2}{(\lambda + \cos \theta_{cm})^2} = \frac{1 + 2\lambda \cos \theta_{cm} + \lambda^2}{(\lambda + \cos \theta_{cm})^2} \\ &\Rightarrow \cos \theta_{lab} = \frac{\lambda + \cos \theta_{cm}}{\sqrt{1 + 2\lambda \cos \theta_{cm} + \lambda^2}} \\ \Rightarrow \frac{d(\cos \theta_{lab})}{d(\cos \theta_{cm})} &= \frac{\sqrt{1 + 2\lambda \cos \theta_{cm} + \lambda^2} - \frac{\lambda(\lambda + \cos \theta_{cm})}{\sqrt{1 + 2\lambda \cos \theta_{cm} + \lambda^2}}}{(1 + 2\lambda \cos \theta_{cm} + \lambda^2)^{\frac{3}{2}}} = \frac{1 + 2\lambda \cos \theta_{cm} + \lambda^2 - \lambda^2 - \lambda \cos \theta_{cm}}{(1 + 2\lambda \cos \theta_{cm} + \lambda^2)^{\frac{3}{2}}} \\ &\Rightarrow \frac{d(\cos \theta_{lab})}{d(\cos \theta_{cm})} = \frac{1 + \lambda \cos \theta_{cm}}{(1 + 2\lambda \cos \theta_{cm} + \lambda^2)^{\frac{3}{2}}} \end{aligned}$$

From which we finally obtain:

$$\left( \frac{d\sigma}{d\Omega} \right)_{lab} = \left( \frac{d\sigma}{d\Omega} \right)_{cm} \frac{d\Omega_{cm}}{d\Omega_{lab}} = \left( \frac{d\sigma}{d\Omega} \right)_{cm} \frac{1 + \lambda \cos \theta_{cm}}{(1 + 2\lambda \cos \theta_{cm} + \lambda^2)^{\frac{3}{2}}}$$

### Problem 4.2

Using the notation from Taylor's book we have:

$$\sigma(d\Omega \leftarrow \phi) = \frac{d\Omega}{(2\pi m)^2} \int d^2\rho \, d^3\bar{p} \, d^3p' \, d^3p'' \, p^2 dp \, \delta(E_p - E_{p'}) \, \delta(E_p - E_{p''}) \, f^*(\mathbf{p} \leftarrow \mathbf{p}') \, f^*(\mathbf{p} \leftarrow \mathbf{p}'') \, \Psi^*(\bar{\mathbf{p}}, \mathbf{p}') \, \Psi^*(\bar{\mathbf{p}}, \mathbf{p}'')$$

Let us now look at the integral:

$$\begin{aligned} \int d^2\rho \, \Psi^*(\bar{\mathbf{p}}, \mathbf{p}') \, \Psi^*(\bar{\mathbf{p}}, \mathbf{p}'') &= \int d^2\rho \, e^{i\rho \cdot (\mathbf{p}' - \mathbf{p}'')} \phi_1^*(\mathbf{p}'_1) \phi_2^*(\mathbf{p}'_2) \phi_1(\mathbf{p}''_1) \phi_2(\mathbf{p}''_2) \\ &= (2\pi)^2 \delta_2(\mathbf{p}'_{1\perp} - \mathbf{p}''_{1\perp}) \phi_1^*(\mathbf{p}'_1) \phi_2^*(\mathbf{p}'_2) \phi_1(\mathbf{p}''_1) \phi_2(\mathbf{p}''_2) \end{aligned}$$

Due to the properties of the  $\delta$ -function we can write:

$$\delta(E_p - E_{p'}) \delta(E_p - E_{p''}) = \delta(E_p - E_{p'}) \delta(E_{p'} - E_{p''})$$

First in the CM frame the total momentum of both particles is strongly peaked about zero measurement (see Taylor), thus  $\mathbf{p}_1 = -\mathbf{p}_2$ , which means that there is a specific momentum where  $\phi_2$  is a small appreciably different from zero, which makes us write  $\phi_2^*(\mathbf{p}'_2) \phi_2(\mathbf{p}''_2) \approx |\phi_2(\mathbf{p}'_2)|$  (this step is to be performed after calculating the integral over  $d^3p''$ ). Second in this case measurement of  $\mathbf{p}_1 = \mathbf{p}'$ , thus we can write everywhere  $\mathbf{p}'$  instead of  $\mathbf{p}_1$ . Third the energy  $E_p = \frac{p^2}{2m}$ , from which using the properties of the  $\delta$ -functions:

$$\delta(\mathbf{p}'_{1\perp} - \mathbf{p}''_{1\perp}) \delta\left(\frac{\mathbf{p}'^2}{2m} - \frac{\mathbf{p}''^2}{2m}\right) = 2m \delta(\mathbf{p}'_{\perp} - \mathbf{p}''_{\perp}) \delta\left((p'_{\parallel} + p''_{\parallel})(p'_{\parallel} - p''_{\parallel})\right)$$

We assume that the wavefunctions are sufficiently narrow so that the points corresponding to  $p'_{\parallel} = -p''_{\parallel}$  do not contribute to the integral, so now when we integrate over  $d^3 p''$  we obtain:

$$\sigma(d\Omega \leftarrow \phi) = d\Omega \int d^3 \bar{p} d^3 p' p^2 dp \frac{1}{p'_{\parallel}} \delta((\mathbf{p} + \mathbf{p}') \cdot (\mathbf{p} - \mathbf{p}')) |f(\mathbf{p} \leftarrow \mathbf{p}') \phi_1(\mathbf{p}') \phi(\mathbf{p}'_2)|^2$$

We use similar arguments to above and evaluate:

$$\sigma(d\Omega \leftarrow \phi) = d\Omega \int d^3 \bar{p} d^3 p' \frac{p'}{p'_{\parallel}} |f(\mathbf{p} \leftarrow \mathbf{p}') \phi_1(\mathbf{p}') \phi(\mathbf{p}'_2)|^2$$

Given that the function change  $f$  changes slowly enough with respect to the peak of the wavefunction we can take it out of the integral and obtain:

$$\sigma(d\Omega \leftarrow \phi) = d\Omega |f(\mathbf{p} \leftarrow \mathbf{p}')|^2 \int d^3 \bar{p} d^3 p' |\Psi(\bar{\mathbf{p}}, \mathbf{p}')|^2 = d\Omega |f(\mathbf{p} \leftarrow \mathbf{p}')|^2$$

Where for small body angles we have:

$$\frac{d\sigma}{d\Omega}(d\Omega \leftarrow \phi) = |f(\mathbf{p} \leftarrow \mathbf{p}')|^2$$

As for the second part it done by interchanging the indices 1 and 2.

## Chapter 5

### Problem 5.1

When we transform  $\langle \mathbf{p}'_1, \mathbf{p}'_2, \xi' | \mathbf{S} | \mathbf{p}_1, \mathbf{p}_2, \xi \rangle$  into CM frame we get a  $\delta(\overline{\mathbf{p}'} - \overline{\mathbf{p}})$ , which we can factor out. If we neglect the no-scattering term then we can write:

$$\langle \mathbf{p}', \xi' | S | \mathbf{p}, \xi \rangle = \frac{i}{2\pi m} \delta(E_{p'} - E_p) f(\mathbf{p}', \xi' \leftarrow \mathbf{p}, \xi)$$

Now we use that:

$$|\chi\rangle = \sum_{\xi} \chi_{\xi} |\xi\rangle, \quad \langle \chi' | = \sum_{\xi'} \chi_{\xi'}^* \langle \xi |$$

Using this we can expand:

$$\langle \mathbf{p}', \chi' | S | \mathbf{p}, \chi \rangle = \sum_{\xi, \xi'} \chi_{\xi'}^* \chi_{\xi} \langle \mathbf{p}', \xi' | S | \mathbf{p}, \xi \rangle$$

From everything up to now it follows using similar arguments and calculations to those in **Problem 4.2** that we obtain:

$$\frac{d\sigma}{d\Omega}(\mathbf{p}', \chi' \leftarrow \mathbf{p}, \chi) = \left| \sum_{\xi, \xi'} \chi_{\xi'}^* f(\mathbf{p}', \xi' \leftarrow \mathbf{p}, \xi) \chi_{\xi} \right|^2$$

### Problem 5.2

Let the spin operator be  $\mathbf{s}$ . The fact that the Hamiltonian  $H$  is spin-independent means that we have:

$$[\mathbf{s}, H] = 0$$

From this it easily follows that:

$$\left[ \mathbf{s}, e^{-\frac{i}{\hbar} \int H dt} \right] = 0$$

For any limits of integration. Thus it should be true considering the integration from  $-\infty$  to  $\infty$ , so we obtain:

$$[\mathbf{s}, S] = 0$$

Now taking the sandwich between two states we obtain (for brevity in the CM frame) and assuming that  $|\xi\rangle$  are the eigenvectors of  $\mathbf{s}$  with eigenvalues  $\xi$ :

$$\langle \mathbf{p}', \xi' | [\mathbf{s}, S] | \mathbf{p}, \xi \rangle = (\xi' - \xi) \langle \mathbf{p}', \xi' | S | \mathbf{p}, \xi \rangle = 0$$

This means that when  $\xi \neq \xi'$ , we necessarily have:

$$\langle \mathbf{p}', \xi' | S | \mathbf{p}, \xi \rangle = 0$$

From everything said up to now we can see that:

$$\langle \mathbf{p}', \xi' | S | \mathbf{p}, \xi \rangle = \delta_{\xi\xi'} \langle \mathbf{p}' | S | \mathbf{p} \rangle$$

As we can see the second term is independent of the spin, which is a direct consequence of the commutation between the spin operator and the Hamiltonian.

Which shows us that the amplitude matrix has the form  $F(\mathbf{p}' \leftarrow \mathbf{p}) = f(\mathbf{p}' \leftarrow \mathbf{p}) I$ . From this we can look at the differential cross section from an incoming unpolarized beam and look at how the particles are scattered for different spin states:

$$\frac{d\sigma}{d\Omega}(\mathbf{p}', \xi' \leftarrow \mathbf{p}) = \frac{1}{(2s_1 + 1)(2s_2 + 1)} \sum_{\xi} \frac{d\sigma}{d\Omega}(\mathbf{p}', \xi' \leftarrow \mathbf{p}, \xi) = \frac{1}{(2s_1 + 1)(2s_2 + 1)} |f(\mathbf{p}' \leftarrow \mathbf{p})|^2$$

This shows the cross section for different final spins is the same and we can not differentiate the particles.

### Problem 5.3

The differential cross section can be written out as:

$$\begin{aligned} \frac{d\sigma}{d\Omega}(\mathbf{p}', \chi' \leftarrow \mathbf{p}, \chi) &= |\chi'^* F(\mathbf{p}' \leftarrow \mathbf{p}) \chi|^2 = \left| \sum_{\xi, \xi'} \chi_{\xi'}'^* f_{\xi', \xi} \chi_{\xi} \right|^2 = \\ &= \left( |\chi_{\uparrow}^* f_{\uparrow\uparrow} \chi_{\uparrow}|^2 + |\chi_{\uparrow}^* f_{\uparrow\downarrow} \chi_{\downarrow}|^2 + |\chi_{\downarrow}^* f_{\downarrow\uparrow} \chi_{\uparrow}|^2 + |\chi_{\downarrow}^* f_{\downarrow\downarrow} \chi_{\downarrow}|^2 \right) + \\ &+ 2\text{Re} \left( (\chi_{\uparrow}^* \chi_{\uparrow}' \chi_{\uparrow}'^* \chi_{\downarrow} f_{\uparrow\uparrow}^* f_{\uparrow\downarrow}) + (\chi_{\uparrow}^* \chi_{\uparrow}' \chi_{\downarrow}'^* \chi_{\uparrow} f_{\uparrow\uparrow}^* f_{\downarrow\uparrow}) + (\chi_{\uparrow}^* \chi_{\uparrow}' \chi_{\downarrow}'^* \chi_{\downarrow} f_{\uparrow\uparrow}^* f_{\downarrow\downarrow}) \right) + \\ &+ 2\text{Re} \left( (\chi_{\uparrow}^* \chi_{\downarrow}' \chi_{\downarrow}'^* \chi_{\uparrow} f_{\uparrow\downarrow}^* f_{\downarrow\uparrow}) + (\chi_{\uparrow}^* \chi_{\downarrow}' \chi_{\downarrow}'^* \chi_{\downarrow} f_{\uparrow\downarrow}^* f_{\downarrow\downarrow}) + (\chi_{\downarrow}^* \chi_{\uparrow}' \chi_{\uparrow}'^* \chi_{\downarrow} f_{\downarrow\uparrow}^* f_{\downarrow\downarrow}) \right) \end{aligned}$$

We can see that in this equation we have ten different terms, accounting for the 10 different measurements that have to be done.

### Problem 5.4

Similarly to before due to the unitarity of S we have  $S^\dagger S = 1$  and from  $S = 1 + R$ , we obtain:

$$R + R^\dagger = -R^\dagger R$$

Now we take the sandwich with  $\langle \mathbf{p}', \chi' |$  and  $|\mathbf{p}, \chi\rangle$  and expansion of the unit operator in terms of the momentum eigenvectors and spins states we have:

$$\langle \mathbf{p}', \chi' | R | \mathbf{p}, \chi \rangle + (\langle \mathbf{p}, \chi | R | \mathbf{p}', \chi' \rangle)^* = \sum_{\xi''} \int d^3 p'' (\langle \mathbf{p}'', \xi'' | R | \mathbf{p}', \chi' \rangle)^* (\langle \mathbf{p}'', \xi'' | R | \mathbf{p}, \chi \rangle)$$

Now using the expansion for R, and factoring out a common constant factor and a common  $\delta$ -function we finally obtain:

$$f(\mathbf{p}', \chi' \leftarrow \mathbf{p}, \chi) - f^*(\mathbf{p}, \chi \leftarrow \mathbf{p}', \chi') = \frac{i}{2\pi m} \sum_{\xi''} \int d^3 p'' \delta(E_p - E_{p''}) f^*(\mathbf{p}'', \xi'' \leftarrow \mathbf{p}', \chi') f(\mathbf{p}'', \xi'' \leftarrow \mathbf{p}, \chi)$$

Now we consider  $\mathbf{p} = \mathbf{p}'$  and  $\chi = \chi'$  from which we have:

$$f(\mathbf{p}, \chi \leftarrow \mathbf{p}, \chi) - f^*(\mathbf{p}, \chi \leftarrow \mathbf{p}, \chi) = \frac{i}{2\pi m} \sum_{\xi''} \int d^3 p'' \delta(E_p - E_{p''}) f^*(\mathbf{p}'', \xi'' \leftarrow \mathbf{p}, \chi) f(\mathbf{p}'', \xi'' \leftarrow \mathbf{p}, \chi)$$

$$2i\text{Im}(f(\mathbf{p}, \chi \leftarrow \mathbf{p}, \chi)) = \frac{i}{2\pi m} \sum_{\xi''} \int d^3 p'' \delta(E_p - E_{p''}) |f(\mathbf{p}'', \xi'' \leftarrow \mathbf{p}, \chi)|^2$$

$$\text{Im}(f(\mathbf{p}, \chi \leftarrow \mathbf{p}, \chi)) = \frac{1}{4\pi m} \sum_{\xi''} \int d^3 p'' \delta\left(\frac{1}{2m}(p + p'')(p - p'')\right) \frac{d\sigma}{d\Omega}(\mathbf{p}'', \xi'' \leftarrow \mathbf{p}, \chi)$$

$$\text{Im}(f(\mathbf{p}, \chi \leftarrow \mathbf{p}, \chi)) = \frac{p}{4\pi} \sum_{\xi''} \int d\Omega_{p''} \frac{d\sigma}{d\Omega}(\mathbf{p}'', \xi'' \leftarrow \mathbf{p}, \chi) = \frac{p}{4\pi} \sigma(\mathbf{p}, \chi)$$

Finally we obtain the total cross section as:

$$\sigma(\mathbf{p}, \chi) = \frac{4\pi}{p} \text{Im}(f(\mathbf{p}, \chi \leftarrow \mathbf{p}, \chi))$$



## Chapter 6

### Problem 6.1

An antiunitary operator  $W$  is defined by:

$$U(a|\psi_1\rangle) = a^*(U|\psi_1\rangle)$$

$$|\langle W\psi|W\phi\rangle| = |\langle\psi|\phi\rangle|$$

We are going to do this problem in a different order, first we will do (c).

(c) Let the conjugation operator be denoted by  $K$ . If we are to use an orthonormal basis  $\{|0\rangle, |1\rangle, \dots, |n\rangle, \dots\}$ , we can then write:

$$K(a|\psi\rangle) = a^*(K|\psi\rangle)$$

$$|(K\psi, K\phi)| = \left| \sum_{nm} a_n b_m^* (n, m) \right| = \left| \sum_n a_n b_n^* \right| = \left| \sum_n a_n^* b_n \right| = |(\psi, \phi)|$$

From this we can see that  $K$  is antiunitary operator.

a) Any antiunitary operator  $W$  we can write as:

$$W = UK$$

Where  $U$  is some unitary operator. From this we obtain:

$$W|\psi\rangle = UK \sum_{i=0}^{\infty} a_i |i\rangle = \sum_{i=0}^{\infty} a_i^* U|i\rangle$$

From which we have:

$$(W\psi, W\phi) = \sum_{nm} (UKa_n n, UKb_m m) = \sum_{nm} a_n b_m^* (Un, Um) = \sum_{nm} a_n b_m^* (n, m) = \sum_n a_n b_n^* = (\phi, \psi) = (\psi, \phi)^*$$

b) From  $\langle\psi|W^\dagger W|\psi\rangle = \langle\psi|\psi\rangle^* = \langle\psi|\psi\rangle$ , we can conclude that in this case  $W^\dagger W = 1$ . Now from the trick used in the text first letting  $|\psi\rangle = |\phi\rangle + |\chi\rangle$  and then  $|\psi\rangle = |\phi\rangle + i|\chi\rangle$ , We obtain two equations:

$$\begin{cases} \langle\phi|W^\dagger W|\chi\rangle + \langle\chi|W^\dagger W|\phi\rangle = \langle\phi|\chi\rangle + \langle\chi|\phi\rangle \\ \langle\phi|W^\dagger W|\chi\rangle - \langle\chi|W^\dagger W|\phi\rangle = \langle\phi|\chi\rangle - \langle\chi|\phi\rangle \end{cases}$$

Adding them together we have:

$$\langle\phi|W^\dagger W|\chi\rangle = \langle\phi|\chi\rangle$$

Thus we can conclude that:

$$W^\dagger W = 1$$

Similarly to what is done in the book one obtains:

$$WW^\dagger = 1$$

### Problem 6.2

### Problem 6.3

### Problem 6.4

### Problem 6.5

### Problem 6.6

### Problem 6.7

### Problem 6.8

### Problem 6.9

## Chapter 7

## Chapter 8

## Chapter 9

## Chapter 10

## Chapter 11

## Chapter 12

## Chapter 13



## Chapter 14

## Chapter 15

## Chapter 16

## Chapter 17

## Chapter 18

## Chapter 19

## Chapter 20

## Chapter 21



## Chapter 22